SoftwareFoundations/SfLib/Hoare.v
@@ -1,0 +1,23 @@
+(**** Hoare: Hoare Logic ****)
+
+Require Export Imp.
+
+(*** Hoare Logic ***)
+
+(** Assertions **)
+
+Definition Assertion := state -> Prop.
+
+(*
+
+1) The variable X is equal to the integer 3.
+2) The variable X is equal to the metavariable x.
+3) The variable X is less than or equal to the variable Y.
+4) The variable X is equal to 3 or it is less than or equal to the variable Y.
+5) The variable Z squared is less than or equal ot the metavariable x and (Z + 1)^2 is
+   greater than x.
+6) Always holds.
+7) Never holds.
+
+*)
+
